\subsection*{Conditional posterior of $\alpha \mid \ldots$}\label{s:alphapost}
Let $\alpha \sim N(0, \tau_\alpha)$ where $\tau_\alpha$ is a precision term. Then
\begin{align*}
  \pi(\alpha \mid \ldots) &\propto \exp \left\{ -\frac{ 1 }{ 2 } \tau_\alpha \alpha^2 + \sum_{ t = 1 }^T \frac{ 1 }{ 2 } [\bY_t - X_t\beta - \alpha z_t]^T \Omega [\bY_t - X_t\beta - \alpha z_t] \right\} \\
      &\propto \exp \left\{ -\frac{ 1 }{ 2 } [\alpha^2(\tau_\alpha + \sum_{t = 1 }^T z_t^T \Omega z_t^T) - 2 \alpha \sum_{t=1}^T[z_t^T \Omega (\bY_t - X_t \beta) \right\}\\
      &\propto \exp \left\{ -\frac{ 1 }{ 2 } [\tau_\alpha^* \alpha^2 - 2 \mu_\alpha] \right\}
\end{align*}
where 
\begin{align*}
  \mu_\alpha &= \sum_{t = 1}^T z_t^T \Omega (\bY_t - X_t \beta)\\
  \tau_\alpha^* &= t_\alpha + \sum_{t=1}^T z_t^T \Omega z_t.
\end{align*}
Then $\alpha \mid \ldots \sim N(\tau^{*-1}_\alpha \mu_\alpha, \tau^{*-1}_\alpha) $